backends/lean/Aeneas/Std/Scalar/Core.lean
@@ -23,7 +23,7 @@ Because they tend to behave quite differently, we have two classes of machine in
 signed integers, and another for unsigned integers. Inside of each class, we factor out definitions.
 -/
 
-open Result Error
+open RustM Error
 
 /-- Kinds of unsigned integers -/
 inductive UScalarTy where
@@ -592,16 +592,16 @@ def UScalar.tryMkOpt (ty : UScalarTy) (x : Nat) : Option (UScalar ty) :=
     some (UScalar.ofNatCore x (UScalar.check_bounds_imp_inBounds h))
   else none
 
-def UScalar.tryMk (ty : UScalarTy) (x : Nat) : Result (UScalar ty) :=
-  Result.ofOption (tryMkOpt ty x) integerOverflow
+def UScalar.tryMk (ty : UScalarTy) (x : Nat) : RustM (UScalar ty) :=
+  RustM.ofOption (tryMkOpt ty x) integerOverflow
 
 def IScalar.tryMkOpt (ty : IScalarTy) (x : Int) : Option (IScalar ty) :=
   if h:IScalar.check_bounds ty x then
     some (IScalar.ofIntCore x (IScalar.check_bounds_imp_inBounds h))
   else none
 
-def IScalar.tryMk (ty : IScalarTy) (x : Int) : Result (IScalar ty) :=
-  Result.ofOption (tryMkOpt ty x) integerOverflow
+def IScalar.tryMk (ty : IScalarTy) (x : Int) : RustM (IScalar ty) :=
+  RustM.ofOption (tryMkOpt ty x) integerOverflow
 
 theorem UScalar.tryMkOpt_eq (ty : UScalarTy) (x : Nat) :
   match tryMkOpt ty x with
