backends/lean/Aeneas/Tactic/Step/Step.lean
@@ -24,7 +24,7 @@ a bug and doesn't give the proper arguments: this way we make sure tactics like 
 will not crash if there is a bug in the code which adds the pretty equality (this is only useful
 information for the user).
 -/
-@[irreducible] def prettyMonadEq {α : Type u} {β : Type v} (_ : Std.Result α) (_ : β) : Type := Unit
+@[irreducible] def prettyMonadEq {α : Type u} {β : Type v} (_ : Std.RustM α) (_ : β) : Type := Unit
 
 macro:max "[> " "let" y:term " ← " x:term " <]"   : term => `(prettyMonadEq $x $y)
 
@@ -33,7 +33,7 @@ def unexpPrettyMonadEqofNat : Lean.PrettyPrinter.Unexpander | `($_ $x $y) => `([
 
 example (x y z : Std.U32) (_ : [> let z ← x + y <]) : True := by simp
 
-def eq_imp_prettyMonadEq {α : Type u} {β : Type v} (x : Std.Result α) (y : β) : prettyMonadEq x y := by
+def eq_imp_prettyMonadEq {α : Type u} {β : Type v} (x : Std.RustM α) (y : β) : prettyMonadEq x y := by
   unfold prettyMonadEq
   constructor
 
@@ -67,7 +67,7 @@ theorem forall_unit {p : Prop} : (Unit → p) ↔ p := by simp
 attribute [step_simps]
   bind_assoc Std.bind_tc_ok Std.bind_tc_fail Std.bind_tc_div
   /- Those are quite useful to simplify the goal further by eliminating existential quantifiers for instance. -/
-  and_assoc Std.Result.ok.injEq Prod.mk.injEq
+  and_assoc Std.RustM.ok.injEq Prod.mk.injEq
   exists_eq_left exists_eq_left' exists_eq_right exists_eq_right' exists_eq exists_eq' true_and and_true
   Std.WP.spec_ok
   -- This one gets only applied to full applications of `uncurry'`, which are typically revealed after applying `spec_ok`
@@ -1454,7 +1454,7 @@ theorem thm_name (arg1 : ty1) ... (argn : tyn)
     (h_pre1 : precondition_1) ... (h_prem : precondition_m) :
   f arg1 ... argn = ⦃ res1 ... resk => postcondition_1 ∧ ... ∧ postcondition_k ⦄
 ```
-where `f` is a monadic function with type `Result ...`.
+where `f` is a monadic function with type `RustM ...`.
 
 **Ghost Variables:**
 It is possible to write step theorems which use ghost variables, i.e., variables
@@ -1563,7 +1563,7 @@ elab tk:letStep : tactic => do
     Meta.Tactic.TryThis.addSuggestion tk stxArgs' (origSpan? := ← getRef)
 
 namespace Test
-  open Std Result
+  open Std RustM
 
   -- Show the traces:
   -- set_option trace.Step true
@@ -1601,7 +1601,7 @@ x y : UScalar ty
     let* ⟨ z, h1 ⟩ ← *
 
   -- Checking that we properly handle tuple decomposition in post-conditions
-  def addToPair (x : Nat) := Result.ok (x + 1, x + 2)
+  def addToPair (x : Nat) := RustM.ok (x + 1, x + 2)
   theorem  addToPair_spec (x : Nat) : addToPair x ⦃ y z => y = x + 1 ∧ z = x + 2⦄ :=
     by simp [addToPair]
 
@@ -1774,12 +1774,12 @@ info: example
      pspec theorem actually solves it, and where the function is not a constant.
      We also test the case where the function under scrutinee is not a constant. -/
   example {x : U32}
-    (f : U32 → Std.Result Unit) (h : ∀ x, f x ⦃ _ => True ⦄) :
+    (f : U32 → Std.RustM Unit) (h : ∀ x, f x ⦃ _ => True ⦄) :
     f x ⦃ _ => True ⦄ := by
     step
 
   example {x : U32}
-    (f : U32 → Std.Result Unit) (h : ∀ x, f x ⦃ _ => True ⦄) :
+    (f : U32 → Std.RustM Unit) (h : ∀ x, f x ⦃ _ => True ⦄) :
     f x ⦃ _ => True ⦄ := by
     step? says step with h
 
@@ -1804,18 +1804,18 @@ info: example
 error: unsolved goals
 case a
 x y : U32
-f : U32 → U32 → Result U32
+f : U32 → U32 → RustM U32
 hf : ∀ (x y : U32), ↑x < 10 → ↑y < 10 → f x y ⦃ x✝ => True ⦄
 ⊢ ↑x < 10
 
 case a
 x y : U32
-f : U32 → U32 → Result U32
+f : U32 → U32 → RustM U32
 hf : ∀ (x y : U32), ↑x < 10 → ↑y < 10 → f x y ⦃ x✝ => True ⦄
 ⊢ ↑y < 10
   -/
   #guard_msgs in
-  example {x y} (f : U32 → U32 → Result U32) (hf : ∀ x y, x.val < 10 → y.val < 10 → f x y ⦃ _ => True⦄) :
+  example {x y} (f : U32 → U32 → RustM U32) (hf : ∀ x y, x.val < 10 → y.val < 10 → f x y ⦃ _ => True⦄) :
     f x y ⦃ _ => True ⦄ := by
     step
 
@@ -1830,11 +1830,11 @@ hf : ∀ (x y : U32), ↑x < 10 → ↑y < 10 → f x y ⦃ x✝ => True ⦄
   end
 
   mutual
-    def Tree.size (t : Tree) : Std.Result Int :=
+    def Tree.size (t : Tree) : Std.RustM Int :=
       match t with
       | .mk trees => trees.size
 
-    def Trees.size (t : Trees) : Std.Result Int :=
+    def Trees.size (t : Trees) : Std.RustM Int :=
       match t with
       | .nil => ok 0
       | .cons t t' => do
@@ -1864,7 +1864,7 @@ hf : ∀ (x y : U32), ↑x < 10 → ↑y < 10 → f x y ⦃ x✝ => True ⦄
   end
 
   -- Testing step on theorems containing local let-bindings
-  def add (x y : U32) : Std.Result U32 := x + y
+  def add (x y : U32) : Std.RustM U32 := x + y
 
   section
     /- Testing step on theorems containing local let-bindings as well as
@@ -1876,7 +1876,7 @@ hf : ∀ (x y : U32), ↑x < 10 → ↑y < 10 → f x y ⦃ x✝ => True ⦄
       step with U32.add_spec.step_spec
       scalar_tac
 
-    def add1 (x y : U32) : Std.Result U32 := do
+    def add1 (x y : U32) : Std.RustM U32 := do
       let z ← x + y
       z + z
 
@@ -1914,10 +1914,10 @@ x y : U32
 end Test
 
 namespace Test
-  open Std Result
+  open Std RustM
 
   variable {α} (P : ℕ → List α → Prop)
-  variable (f : List α → Std.Result Bool)
+  variable (f : List α → Std.RustM Bool)
   variable (f_spec : ∀ l i, P i l → f l ⦃ _ => True ⦄)
 
   example {i} (l : List α) (h : P i l) :
@@ -1926,14 +1926,14 @@ namespace Test
 
   /- Step using a term -/
   example {x: U32}
-    (f : U32 → Std.Result Unit)
+    (f : U32 → Std.RustM Unit)
     (h : ∀ x, f x ⦃ _ => True ⦄):
       f x ⦃ () => True ⦄ := by
       step? with (show ∀ x, f x ⦃ _ => True ⦄ by exact h) says step with(show ∀ x, f x ⦃ _ => True ⦄ by exact h)
 end Test
 
 namespace Test
-  open Std Result
+  open Std RustM
 
   /- Step using a term -/
   example (x y : U32) (h : 2 * x.val + 2 * y.val ≤ U32.max) :
@@ -1993,7 +1993,7 @@ info: example
 error: unsolved goals
 case a
 x : U32
-f : U32 → Result U32
+f : U32 → RustM U32
 h : ∀ (x : U32), f x ⦃ y => ∃ z > 0, ↑y = ↑x + z ⦄
 y : ℕ
 z : U32
@@ -2002,12 +2002,12 @@ _✝ : ↑z = ↑x + y
 ⊢ ↑z > ↑x
   -/
   #guard_msgs in
-  example (x : U32) (f : U32 → Result U32) (h : ∀ x, f x ⦃ y => ∃ z, z > 0 ∧ y.val = x.val + z ⦄) :
+  example (x : U32) (f : U32 → RustM U32) (h : ∀ x, f x ⦃ y => ∃ z, z > 0 ∧ y.val = x.val + z ⦄) :
     f x ⦃ y => y.val > x.val ⦄ := by
     step as ⟨ y, z ⟩
 
   /- Inhabited -/
-  def get (x : Option α) : Result α :=
+  def get (x : Option α) : RustM α :=
     match x with
     | none => fail .panic
     | some x => ok x
@@ -2043,7 +2043,7 @@ z_post : ↑z = ↑x + ↑y
   /--
 error: unsolved goals
 case a
-zero : Slice U32 → Result (Slice U32)
+zero : Slice U32 → RustM (Slice U32)
 zero_spec :
   ∀ (s : Slice U32), zero s ⦃ s' => ∃ (h : s'.length = s.length), ∀ (i : ℕ) (x : i < s.length), s'[i] = 0#u32 ⦄
 s s' : Slice U32
@@ -2055,7 +2055,7 @@ h1 : ∀ (i : ℕ) (x : i < s.length), s'[i] = 0#u32
     x✝ => True ⦄
   -/
   #guard_msgs in
-  example (zero : Slice U32 → Result (Slice U32))
+  example (zero : Slice U32 → RustM (Slice U32))
     (zero_spec : ∀ s, zero s ⦃ s' =>
       ∃ (h : s'.length = s.length),
       (∀ i, (_ : i < s.length) → s'[i]'(by grind) = 0#u32) ⦄)
@@ -2077,7 +2077,7 @@ h1 : ∀ (i : ℕ) (x : i < s.length), s'[i] = 0#u32
   namespace Ntt
     def wfArray (_ : Array U16 256#usize) : Prop := True
 
-    def nttLayer (a : Array U16 256#usize) (_k : Usize) (_len : Usize) : Std.Result (Array U16 256#usize) := ok a
+    def nttLayer (a : Array U16 256#usize) (_k : Usize) (_len : Usize) : Std.RustM (Array U16 256#usize) := ok a
 
     def toPoly (a : Array U16 256#usize) : List U16 := a.val
 
@@ -2096,7 +2096,7 @@ h1 : ∀ (i : ℕ) (x : i < s.length), s'[i] = 0#u32
         wfArray peSrc' ⦄ := by
       simp [wfArray, nttLayer, toPoly, Spec.nttLayer]
 
-    def ntt (x : Array U16 256#usize) : Std.Result (Array U16 256#usize) := do
+    def ntt (x : Array U16 256#usize) : Std.RustM (Array U16 256#usize) := do
       let x ← nttLayer x 1#usize 128#usize
       let x ← nttLayer x 2#usize 64#usize
       let x ← nttLayer x 4#usize 32#usize
@@ -2156,7 +2156,7 @@ h1 : ∀ (i : ℕ) (x : i < s.length), s'[i] = 0#u32
 
   namespace DspecTests
   -- This section has tests for dspec.
-  def simple_diverge (x : Std.I32) : Result Std.I32 := do
+  def simple_diverge (x : Std.I32) : RustM Std.I32 := do
     if x = 0#i32
     then ok 10#i32
     else
@@ -2182,7 +2182,7 @@ h1 : ∀ (i : ℕ) (x : i < s.length), s'[i] = 0#u32
           step
           simp [*]
 
-  def simple_diverge_2 (x y : Std.I32) : Result Std.I32 := do
+  def simple_diverge_2 (x y : Std.I32) : RustM Std.I32 := do
     if x = 0#i32
     then ok 10#i32
     else
@@ -2190,7 +2190,7 @@ h1 : ∀ (i : ℕ) (x : i < s.length), s'[i] = 0#u32
       simple_diverge_2 i1 i1
   partial_fixpoint
 
-  def simple_converge (x : Std.I32) : Result Std.I32 := do
+  def simple_converge (x : Std.I32) : RustM Std.I32 := do
     if x = 0#i32
     then ok 10#i32
     else ok 10#i32
@@ -2238,7 +2238,7 @@ h1 : ∀ (i : ℕ) (x : i < s.length), s'[i] = 0#u32
     simp [*]
 
   -- test lifting an assumption
-  example (f : I32 → Result I32)
+  example (f : I32 → RustM I32)
     (h : ∀ x, (f x) ⦃fun y => y.val = 10⦄)
     :
     ( do let x ← f 1#i32
