backends/lean/Aeneas/Std/Core/Default.lean
@@ -4,9 +4,9 @@ namespace Aeneas.Std
 
 @[rust_trait "core::default::Default"]
 structure core.default.Default (Self : Type u) where
-  default : Result Self
+  default : RustM Self
 
 @[rust_fun "core::default::{core::default::Default<bool>}::default"]
-def core.default.DefaultBool.default : Result Bool := .ok false
+def core.default.DefaultBool.default : RustM Bool := .ok false
 
 end Aeneas.Std
