backends/lean/Aeneas/Std/Core/Ptr.lean
@@ -82,7 +82,7 @@ structure core.alloc.layout.Layout where
 
 @[rust_trait "core::alloc::global::GlobalAlloc"]
 structure core.alloc.global.GlobalAlloc (Self : Type) where
-  alloc : Self → core.alloc.layout.Layout → Result (MutRawPtr U8)
-  dealloc : Self → MutRawPtr U8 → core.alloc.layout.Layout → Result Unit
+  alloc : Self → core.alloc.layout.Layout → RustM (MutRawPtr U8)
+  dealloc : Self → MutRawPtr U8 → core.alloc.layout.Layout → RustM Unit
 
 end Aeneas.Std
