backends/lean/Aeneas/Std/RawPtr.lean
@@ -27,7 +27,7 @@ instance {ty} : IsScalar (IScalar ty) where
 
 -- TODO: we can properly define this once we have separation logic
 def RawPtr.cast_scalar {T} {M} (T' : Type) (M' : Mutability) [IsScalar T] [IsScalar T'] (_ : RawPtr T M) :
-  Result (RawPtr T' M') :=
+  RustM (RawPtr T' M') :=
   .fail .undef
 
 end Aeneas.Std
