backends/lean/Aeneas/Std/Scalar/Fmt.lean
@@ -5,43 +5,43 @@ namespace Aeneas.Std
 
 @[rust_fun "core::fmt::num::{core::fmt::LowerHex<u16>}::fmt"]
 def core.fmt.num.LowerHexU16.fmt (_ : U16) (fmt : core.fmt.Formatter) :
-  Result (core.result.Result Unit core.fmt.Error × core.fmt.Formatter) :=
+  RustM (core.result.Result Unit core.fmt.Error × core.fmt.Formatter) :=
   -- TODO: this is a simplistic model
   .ok (.Ok (), fmt)
 
 @[rust_fun "core::fmt::num::{core::fmt::Debug<u8>}::fmt"]
 def core.fmt.num.DebugU8.fmt (_ : U8) (fmt : core.fmt.Formatter) :
-  Result (core.result.Result Unit core.fmt.Error × core.fmt.Formatter) :=
+  RustM (core.result.Result Unit core.fmt.Error × core.fmt.Formatter) :=
   -- TODO: this is a simplistic model
   .ok (.Ok (), fmt)
 
 @[rust_fun "core::fmt::num::{core::fmt::Debug<u16>}::fmt"]
 def core.fmt.num.DebugU16.fmt (_ : U16) (fmt : core.fmt.Formatter) :
-  Result (core.result.Result Unit core.fmt.Error × core.fmt.Formatter) :=
+  RustM (core.result.Result Unit core.fmt.Error × core.fmt.Formatter) :=
   -- TODO: this is a simplistic model
   .ok (.Ok (), fmt)
 
 @[rust_fun "core::fmt::num::{core::fmt::Debug<u32>}::fmt"]
 def core.fmt.num.DebugU32.fmt (_ : U32) (fmt : core.fmt.Formatter) :
-  Result (core.result.Result Unit core.fmt.Error × core.fmt.Formatter) :=
+  RustM (core.result.Result Unit core.fmt.Error × core.fmt.Formatter) :=
   -- TODO: this is a simplistic model
   .ok (.Ok (), fmt)
 
 @[rust_fun "core::fmt::num::{core::fmt::Debug<u64>}::fmt"]
 def core.fmt.num.DebugU64.fmt (_ : U64) (fmt : core.fmt.Formatter) :
-  Result (core.result.Result Unit core.fmt.Error × core.fmt.Formatter) :=
+  RustM (core.result.Result Unit core.fmt.Error × core.fmt.Formatter) :=
   -- TODO: this is a simplistic model
   .ok (.Ok (), fmt)
 
 @[rust_fun "core::fmt::num::{core::fmt::Debug<u128>}::fmt"]
 def core.fmt.num.DebugU128.fmt (_ : U128) (fmt : core.fmt.Formatter) :
-  Result (core.result.Result Unit core.fmt.Error × core.fmt.Formatter) :=
+  RustM (core.result.Result Unit core.fmt.Error × core.fmt.Formatter) :=
   -- TODO: this is a simplistic model
   .ok (.Ok (), fmt)
 
 @[rust_fun "core::fmt::num::{core::fmt::Debug<usize>}::fmt"]
 def core.fmt.num.DebugUsize.fmt (_ : Usize) (fmt : core.fmt.Formatter) :
-  Result (core.result.Result Unit core.fmt.Error × core.fmt.Formatter) :=
+  RustM (core.result.Result Unit core.fmt.Error × core.fmt.Formatter) :=
   -- TODO: this is a simplistic model
   .ok (.Ok (), fmt)
 
@@ -77,37 +77,37 @@ def core.fmt.DebugUsize : core.fmt.Debug Usize := {
 
 @[rust_fun "core::fmt::num::{core::fmt::Debug<i8>}::fmt"]
 def core.fmt.num.DebugI8.fmt (_ : I8) (fmt : core.fmt.Formatter) :
-  Result (core.result.Result Unit core.fmt.Error × core.fmt.Formatter) :=
+  RustM (core.result.Result Unit core.fmt.Error × core.fmt.Formatter) :=
   -- TODO: this is a simplistic model
   .ok (.Ok (), fmt)
 
 @[rust_fun "core::fmt::num::{core::fmt::Debug<i16>}::fmt"]
 def core.fmt.num.DebugI16.fmt (_ : I16) (fmt : core.fmt.Formatter) :
-  Result (core.result.Result Unit core.fmt.Error × core.fmt.Formatter) :=
+  RustM (core.result.Result Unit core.fmt.Error × core.fmt.Formatter) :=
   -- TODO: this is a simplistic model
   .ok (.Ok (), fmt)
 
 @[rust_fun "core::fmt::num::{core::fmt::Debug<i32>}::fmt"]
 def core.fmt.num.DebugI32.fmt (_ : I32) (fmt : core.fmt.Formatter) :
-  Result (core.result.Result Unit core.fmt.Error × core.fmt.Formatter) :=
+  RustM (core.result.Result Unit core.fmt.Error × core.fmt.Formatter) :=
   -- TODO: this is a simplistic model
   .ok (.Ok (), fmt)
 
 @[rust_fun "core::fmt::num::{core::fmt::Debug<i64>}::fmt"]
 def core.fmt.num.DebugI64.fmt (_ : I64) (fmt : core.fmt.Formatter) :
-  Result (core.result.Result Unit core.fmt.Error × core.fmt.Formatter) :=
+  RustM (core.result.Result Unit core.fmt.Error × core.fmt.Formatter) :=
   -- TODO: this is a simplistic model
   .ok (.Ok (), fmt)
 
 @[rust_fun "core::fmt::num::{core::fmt::Debug<i128>}::fmt"]
 def core.fmt.num.DebugI128.fmt (_ : I128) (fmt : core.fmt.Formatter) :
-  Result (core.result.Result Unit core.fmt.Error × core.fmt.Formatter) :=
+  RustM (core.result.Result Unit core.fmt.Error × core.fmt.Formatter) :=
   -- TODO: this is a simplistic model
   .ok (.Ok (), fmt)
 
 @[rust_fun "core::fmt::num::{core::fmt::Debug<isize>}::fmt"]
 def core.fmt.num.DebugIsize.fmt (_ : Isize) (fmt : core.fmt.Formatter) :
-  Result (core.result.Result Unit core.fmt.Error × core.fmt.Formatter) :=
+  RustM (core.result.Result Unit core.fmt.Error × core.fmt.Formatter) :=
   -- TODO: this is a simplistic model
   .ok (.Ok (), fmt)
 
